Download Link: https://assignmentchef.com/product/solved-convert-the-following-boolean-equation
<br>
<ol>

 <li>Convert the following Boolean equation to canonical sum-of-minterms form:</li>

</ol>

F(a,b,c) = abc’ + a’c

2.  Fill out the truth table for the equation F = abc + a’b’c + a’bc

Input either 0 or 1 in each text field.

a b c

0 0 0

0 0 1

0 1 0

0 1 1

1 0 0

1 0 1

1 1 0

1 1 1

3. Convert the following Boolean equation to canonical sum-of-minterms form:

F(a,b,c) = abc’ + ab’c

4.  Fill out the truth table for the equation F = (a’ + b) * c

Input either 0 or 1 in each text field.

a b c

0 0 0

0 0 1

0 1 0

0 1 1

1 0 0

1 0 1

1 1 0

1 1 1

5.  Convert the following Boolean equation to canonical sum-of-minterms form:

F(a,b,c) = b’c’

6. Fill out the truth table for the equation F = a

Input either 0 or 1 in each text field.

a b c F = a

0 0 0

0 0 1

0 1 0

0 1 1

1 0 0

1 0 1

1 1 0

1 1 1

7.  Convert the following Boolean equation to canonical sum-of-minterms form:

F(a,b,c) = abc + ab + bc